minor

src/program_proof/wal/invariant.v
@@ -123,13 +123,14 @@ Definition is_mem_memLog memLog txns memStart_txn_id : Prop :=
   has_updates memLog.(slidingM.log) (drop memStart_txn_id txns) ∧
   (Forall (λ pos, int.val pos ≤ slidingM.memEnd memLog) txns.*1).
 
-Definition memLog_linv_pers_core γ (σ: slidingM.t) (diskEnd: u64) diskEnd_txn_id nextDiskEnd_txn_id (txns: list (u64 * list update.t)) : iProp Σ :=
+Definition memLog_linv_pers_core γ (σ: slidingM.t) (diskEnd: u64) diskEnd_txn_id nextDiskEnd_txn_id (txns: list (u64 * list update.t)) (logger_pos : u64) : iProp Σ :=
   (∃ (memStart_txn_id: nat),
       "%Htxn_id_ordering" ∷ ⌜(memStart_txn_id ≤ diskEnd_txn_id ≤ nextDiskEnd_txn_id)%nat⌝ ∗
       "#HmemStart_txn" ∷ txn_pos γ memStart_txn_id σ.(slidingM.start) ∗
       "%HdiskEnd_txn" ∷ ⌜is_highest_txn txns diskEnd_txn_id diskEnd⌝ ∗
       "#HnextDiskEnd_txn" ∷ txn_pos γ nextDiskEnd_txn_id σ.(slidingM.mutable) ∗
       "#HmemEnd_txn" ∷ txn_pos γ (length txns - 1)%nat (slidingM.endPos σ) ∗
+      "%HloggerPosOK" ∷ ⌜int.val diskEnd ≤ int.val logger_pos ≤ int.val σ.(slidingM.mutable)⌝ ∗
       (* Here we establish what the memLog contains, which is necessary for reads
       to work (they read through memLogMap, but the lock invariant establishes
       that this matches memLog). *)
@@ -149,8 +150,8 @@ Definition memLog_linv_pers_core γ (σ: slidingM.t) (diskEnd: u64) diskEnd_txn_
           (subslice (S diskEnd_txn_id) (S nextDiskEnd_txn_id) txns)⌝
   ).
 
-Global Instance memLog_linv_pers_core_persistent γ σ diskEnd diskEnd_txn_id nextDiskEnd_txn_id txns:
-  Persistent (memLog_linv_pers_core γ σ diskEnd diskEnd_txn_id nextDiskEnd_txn_id txns).
+Global Instance memLog_linv_pers_core_persistent γ σ diskEnd diskEnd_txn_id nextDiskEnd_txn_id txns logger_pos:
+  Persistent (memLog_linv_pers_core γ σ diskEnd diskEnd_txn_id nextDiskEnd_txn_id txns logger_pos).
 Proof. apply _. Qed.
 
 Definition memLog_linv γ (σ: slidingM.t) (diskEnd: u64) diskEnd_txn_id : iProp Σ :=
@@ -694,14 +695,15 @@ Proof.
       lia.
 Qed.
 
-Lemma memLog_linv_pers_core_strengthen γ σ diskEnd diskEnd_txn_id nextDiskEnd_txn_id txns:
-  (memLog_linv_pers_core γ σ diskEnd diskEnd_txn_id nextDiskEnd_txn_id txns) -∗
+Lemma memLog_linv_pers_core_strengthen γ σ diskEnd diskEnd_txn_id nextDiskEnd_txn_id txns (logger_pos : u64):
+  (memLog_linv_pers_core γ σ diskEnd diskEnd_txn_id nextDiskEnd_txn_id txns logger_pos) -∗
   (ghost_var γ.(txns_name) (1/2) txns) -∗
   (map_ctx γ.(stable_txn_ids_name) (1/2) (<[nextDiskEnd_txn_id := tt]> ∅)) -∗
   (nextDiskEnd_txn_id [[γ.(stable_txn_ids_name)]]↦ro ()) -∗
+  (ghost_var γ.(logger_pos_name) (1 / 2) logger_pos) -∗
   memLog_linv γ σ diskEnd diskEnd_txn_id.
 Proof.
-  iNamed 1. iIntros "H Hm Hs". iExists _, _, _, _. iFrame. iFrame "#". iFrame "%".
+  iNamed 1. iIntros "H Hm Hs Hl". iExists _, _, _, _, _. iFrame. iFrame "#". iFrame "%".
   iPureIntro. intros.
   rewrite lookup_insert_ne; last by lia.
   rewrite lookup_empty. done.
